[move-prover] Separate resource memory by type.
This PR implements separation of resource memory by type instead of using one global memory variable. This makes live for Z3 simpler because

- Automatic modifies analysis is more precise and only those memories are marked as modified which are actually touched on a per-type basis.
- Less aliasing has to be considered which likley reduces case splitting.

As a result, all timeout problems in existing modules could be resolved (except one related to loops). Note that this doesn't necessarily mean yet we have more verified, because many of the functions timing out have no specification conditions yet, but where just calling other functions which have. The overall performance improvement is hard to measure, but some problems which timed out now pass in seconds, and LibraAccount verification has become faster by about 40%.

The separation of memory is possible because:

- Move does not allow for `borrow_global<T>` where T is a type parameter. The outest type in borrow must be concrete. This allows us to statically know the memory being queried.
- The new memory model made it particular easy to implement this, because WriteRef on an arbitrary reference does not commit to the global state yet. Rather commit happens only on the root, where we know the effected memory statically.

This PR also cleans up some stuff, removing Sender and transaction support, and fixing a few more loose ends.

language/move-prover/src/boogie_helpers.rs
@@ -134,6 +134,16 @@ pub fn boogie_struct_type_value(
     )
 }
 
+/// Creates the name of the resource memory for the given struct.
+pub fn boogie_resource_memory_name(
+    env: &GlobalEnv,
+    module_id: ModuleId,
+    struct_id: StructId,
+) -> String {
+    let struct_env = env.get_module(module_id).into_struct(struct_id);
+    format!("{}_memory", boogie_struct_name(&struct_env))
+}
+
 /// Create boogie type value list, separated by comma.
 pub fn boogie_type_values(env: &GlobalEnv, args: &[Type]) -> String {
     args.iter()
@@ -141,10 +151,22 @@ pub fn boogie_type_values(env: &GlobalEnv, args: &[Type]) -> String {
         .join(", ")
 }
 
+/// Creates a type value array for given types.
+pub fn boogie_type_value_array(env: &GlobalEnv, args: &[Type]) -> String {
+    if args.is_empty() {
+        return "$EmptyTypeValueArray".to_string();
+    }
+    let mut map = String::from("$MapConstTypeValue($DefaultTypeValue())");
+    for (i, arg) in args.iter().enumerate() {
+        map = format!("{}[{} := {}]", map, i, boogie_type_value(env, arg));
+    }
+    format!("$TypeValueArray({}, {})", map, args.len())
+}
+
 /// Return boogie type for a local with given signature token.
 pub fn boogie_local_type(ty: &Type) -> String {
     if ty.is_reference() {
-        "$Reference".to_string()
+        "$Mutation".to_string()
     } else {
         "$Value".to_string()
     }
